prop_merge progress

fqueue2.fst
@@ -1097,6 +1097,10 @@ val prop_merge001 : ltr: ae
                                               mem x (absmerge ltr atr btr).l && get_id x <> get_id d && matched x d (absmerge ltr atr btr))))
                                               (absmerge ltr atr btr).l))))
 
+#reset-options
+
+#set-options "--query_stats --initial_fuel 10 --ifuel 10 --initial_ifuel 10 --fuel 10 --z3rlimit 1000000"
+
 let prop_merge001 ltr l atr a btr b =
   axiom_ae ltr; axiom_ae atr; axiom_ae btr; axiom_ae (union ltr atr); axiom_ae (union ltr btr);
   prop_merge01 ltr l atr a btr b;
@@ -1139,7 +1143,7 @@ let prop_merge002 ltr l atr a btr b =
   axiom_ae ltr; axiom_ae atr; axiom_ae btr; axiom_ae (union ltr atr); axiom_ae (union ltr btr);
   prop_merge01 ltr l atr a btr b;
   let tr = absmerge ltr atr btr in
-  let s0 = merge ltr l atr a btr b in
+  let s0 = merge ltr l atr a btr b in admit();
   let enq_list = filter_op (fun x -> is_enqueue x && mem x tr.l && not
                              (exists_mem tr.l (fun d -> is_dequeue d && mem d tr.l && mem x tr.l && get_id x <> get_id d && matched x d tr))) tr.l in
 
@@ -1187,9 +1191,52 @@ let prop_merge0 ltr l atr a btr b =
   axiom_ae ltr; axiom_ae atr; axiom_ae btr; axiom_ae (union ltr atr); axiom_ae (union ltr btr);
   prop_merge01 ltr l atr a btr b; prop_merge001 ltr l atr a btr b; prop_merge002 ltr l atr a btr b;
   let tr = absmerge ltr atr btr in
+  let s0 = merge ltr l atr a btr b in admit();
+  let enq_list = filter_op (fun x -> is_enqueue x && mem x tr.l && not
+                             (exists_mem tr.l (fun d -> is_dequeue d && mem d tr.l && mem x tr.l && get_id x <> get_id d && matched x d tr))) tr.l in
+
+  assert(forall e. mem e enq_list ==> memq (get_id e, get_ele e) s0);
+  assert(forall e. memq e s0 ==> mem (fst e, Enqueue (snd e)) enq_list);
+  assert(forall_mem (tolist s0) (fun e -> mem (fst e, Enqueue (snd e)) enq_list) &&
+                    forall_mem enq_list (fun x -> mem x tr.l && is_enqueue x && mem ((get_id x), (get_ele x)) (tolist s0)));
+  ()
+
+val prop_merge1 : ltr: ae
+                -> l:s
+                -> atr:ae
+                -> a:s
+                -> btr:ae
+                -> b:s
+                -> Lemma (requires ((forall e. mem e ltr.l ==> not (member (get_id e) atr.l)) /\
+                                   (forall e. mem e ltr.l ==> not (member (get_id e) btr.l)) /\
+                                   (forall e. mem e atr.l ==> not (member (get_id e) btr.l)) /\
+                                   (forall e e1. (memq e a /\ memq e1 l /\ (fst e = fst e1)) ==> (snd e = snd e1)) /\
+                                   (forall e e1. (memq e b /\ memq e1 l /\ (fst e = fst e1)) ==> (snd e = snd e1)) /\
+                                   (forall e e1. (mem e ltr.l /\ mem e1 atr.l ==> get_id e < get_id e1)) /\
+                                   (forall e e1. (mem e ltr.l /\ mem e1 btr.l ==> get_id e < get_id e1)) /\
+                                   (sim ltr l /\ sim (union ltr atr) a /\ sim (union ltr btr) b) /\
+                                   (forall e. mem_id e (diff_s (tolist a) (tolist l)) ==> not (mem_id e (diff_s (tolist b) (tolist l)))) /\
+                                   (forall e. mem_id e (diff_s (tolist b) (tolist l)) ==> not (mem_id e (diff_s (tolist a) (tolist l))))))
+                       (ensures (sim1 (absmerge ltr atr btr) (merge ltr l atr a btr b)))
+
+let prop_merge1 ltr l atr a btr b =
+  axiom_ae ltr; axiom_ae atr; axiom_ae btr; axiom_ae (union ltr atr); axiom_ae (union ltr btr);
+  prop_merge01 ltr l atr a btr b; prop_merge0 ltr l atr a btr b;
+  let tr = absmerge ltr atr btr in
   let s0 = merge ltr l atr a btr b in
   let enq_list = filter_op (fun x -> is_enqueue x && mem x tr.l && not
                              (exists_mem tr.l (fun d -> is_dequeue d && mem d tr.l && mem x tr.l && get_id x <> get_id d && matched x d tr))) tr.l in
+
+  // let enq_list1 = filter_op (fun x -> is_enqueue x && mem x ltr.l && not
+  //                            (exists_mem ltr.l (fun d -> is_dequeue d && mem d ltr.l && mem x ltr.l && get_id x <> get_id d && matched x d ltr))) ltr.l in
+
+  // let enq_list2 = filter_op (fun x -> is_enqueue x && mem x (union ltr atr).l && not
+  //                            (exists_mem (union ltr atr).l (fun d -> is_dequeue d && mem d (union ltr atr).l && mem x (union ltr atr).l &&
+  //                                        get_id x <> get_id d && matched x d (union ltr atr)))) (union ltr atr).l in
+
+  // let enq_list3 = filter_op (fun x -> is_enqueue x && mem x (union ltr btr).l && not
+  //                            (exists_mem (union ltr btr).l (fun d -> is_dequeue d && mem d (union ltr btr).l && mem x (union ltr btr).l &&
+  //                                        get_id x <> get_id d && matched x d (union ltr btr)))) (union ltr btr).l in
 
   // let enq_list4 = filter_op (fun x -> is_enqueue x && mem x atr.l && not
   //                            (exists_mem atr.l (fun d -> is_dequeue d && mem d atr.l && mem x atr.l && get_id x <> get_id d && matched x d atr))) atr.l in
@@ -1203,118 +1250,58 @@ let prop_merge0 ltr l atr a btr b =
   //                                        get_id x <> get_id d && matched x d (union ltr atr)))
   //                              && not (exists_mem (union ltr btr).l (fun d -> is_dequeue d && mem d (union ltr btr).l && mem x (union ltr btr).l &&
   //                                        get_id x <> get_id d && matched x d (union ltr btr)))) ltr.l in
-
-  // assert(forall e. (mem e enq_list6) \/ (mem e enq_list4) \/ (mem e enq_list5) ==> mem e enq_list);
-  // assert(forall e. (mem e enq_list6) \/ (mem e enq_list4) \/ (mem e enq_list5) ==> memq (get_id e, get_ele e) s0);
-  // assert(forall e. mem e enq_list ==> ((mem e enq_list4) \/ (mem e enq_list5) \/ (mem e enq_list6)));
-  // assert(forall e. mem e enq_list ==> memq (get_id e, get_ele e) s0);
-
-  // assert(forall e. ((memq e a /\ memq e b /\ memq e l) \/ (mem e (diff_s (tolist a) (tolist l))) \/ (mem e (diff_s (tolist b) (tolist l)))) ==>
-  //                    mem (fst e, Enqueue (snd e)) enq_list);
-  // assert(forall e. ((memq e a /\ memq e b /\ memq e l) \/ (mem e (diff_s (tolist a) (tolist l))) \/ (mem e (diff_s (tolist b) (tolist l)))) <==>
-  //                    memq e s0);
-  // assert(forall e. memq e s0 ==> mem (fst e, Enqueue (snd e)) enq_list);
-  assert(forall_mem (tolist s0) (fun e -> mem (fst e, Enqueue (snd e)) enq_list) && forall_mem enq_list (fun x -> mem x tr.l && is_enqueue x && mem ((get_id x), (get_ele x)) (tolist s0)));
-  ()
-
-// val prop_merge1 : ltr: ae
-//                 -> l:s
-//                 -> atr:ae
-//                 -> a:s
-//                 -> btr:ae
-//                 -> b:s
-//                 -> Lemma (requires ((forall e. mem e ltr.l ==> not (member (get_id e) atr.l)) /\
-//                                    (forall e. mem e ltr.l ==> not (member (get_id e) btr.l)) /\
-//                                    (forall e. mem e atr.l ==> not (member (get_id e) btr.l)) /\
-//                                    (forall e e1. (memq e a /\ memq e1 l /\ (fst e = fst e1)) ==> (snd e = snd e1)) /\
-//                                    (forall e e1. (memq e b /\ memq e1 l /\ (fst e = fst e1)) ==> (snd e = snd e1)) /\
-//                                    (forall e e1. (mem e ltr.l /\ mem e1 atr.l ==> get_id e < get_id e1)) /\
-//                                    (forall e e1. (mem e ltr.l /\ mem e1 btr.l ==> get_id e < get_id e1)) /\
-//                                    (sim ltr l /\ sim (union ltr atr) a /\ sim (union ltr btr) b) /\
-//                                    (forall e. mem_id e (diff_s (tolist a) (tolist l)) ==> not (mem_id e (diff_s (tolist b) (tolist l)))) /\
-//                                    (forall e. mem_id e (diff_s (tolist b) (tolist l)) ==> not (mem_id e (diff_s (tolist a) (tolist l))))))
-//                        (ensures (sim1 (absmerge ltr atr btr) (merge ltr l atr a btr b)))
-
-// let prop_merge1 ltr l atr a btr b =
-//   axiom_ae ltr; axiom_ae atr; axiom_ae btr; axiom_ae (union ltr atr); axiom_ae (union ltr btr);
-//   prop_merge01 ltr l atr a btr b; prop_merge0 ltr l atr a btr b;
-//   let tr = absmerge ltr atr btr in
-//   let s0 = merge ltr l atr a btr b in
-//   let enq_list = filter_op (fun x -> is_enqueue x && mem x tr.l && not
-//                              (exists_mem tr.l (fun d -> is_dequeue d && mem d tr.l && mem x tr.l && get_id x <> get_id d && matched x d tr))) tr.l in
-
-//   // let enq_list1 = filter_op (fun x -> is_enqueue x && mem x ltr.l && not
-//   //                            (exists_mem ltr.l (fun d -> is_dequeue d && mem d ltr.l && mem x ltr.l && get_id x <> get_id d && matched x d ltr))) ltr.l in
-
-//   // let enq_list2 = filter_op (fun x -> is_enqueue x && mem x (union ltr atr).l && not
-//   //                            (exists_mem (union ltr atr).l (fun d -> is_dequeue d && mem d (union ltr atr).l && mem x (union ltr atr).l &&
-//   //                                        get_id x <> get_id d && matched x d (union ltr atr)))) (union ltr atr).l in
-
-//   // let enq_list3 = filter_op (fun x -> is_enqueue x && mem x (union ltr btr).l && not
-//   //                            (exists_mem (union ltr btr).l (fun d -> is_dequeue d && mem d (union ltr btr).l && mem x (union ltr btr).l &&
-//   //                                        get_id x <> get_id d && matched x d (union ltr btr)))) (union ltr btr).l in
-
-//   // let enq_list4 = filter_op (fun x -> is_enqueue x && mem x atr.l && not
-//   //                            (exists_mem atr.l (fun d -> is_dequeue d && mem d atr.l && mem x atr.l && get_id x <> get_id d && matched x d atr))) atr.l in
-
-//   // let enq_list5 = filter_op (fun x -> is_enqueue x && mem x btr.l && not
-//   //                            (exists_mem btr.l (fun d -> is_dequeue d && mem d btr.l && mem x btr.l && get_id x <> get_id d && matched x d btr))) btr.l in
-
-//   // let enq_list6 = filter_op (fun x -> is_enqueue x && mem x ltr.l && not
-//   //                            (exists_mem ltr.l (fun d -> is_dequeue d && mem d ltr.l && mem x ltr.l && get_id x <> get_id d && matched x d ltr))
-//   //                              && not (exists_mem (union ltr atr).l (fun d -> is_dequeue d && mem d (union ltr atr).l && mem x (union ltr atr).l &&
-//   //                                        get_id x <> get_id d && matched x d (union ltr atr)))
-//   //                              && not (exists_mem (union ltr btr).l (fun d -> is_dequeue d && mem d (union ltr btr).l && mem x (union ltr btr).l &&
-//   //                                        get_id x <> get_id d && matched x d (union ltr btr)))) ltr.l in
-//   // assert(forall_mem (enq_list) (fun e -> (forall_mem (filter_op (fun e1 -> get_id e <> get_id e1 && ((tr.vis e e1))) (enq_list))
-//   //                         (fun e1 -> memq ((get_id e), (get_ele e)) s0 && memq ((get_id e1), (get_ele e1)) s0 && get_id e <> get_id e1 &&
-//   //                            order ((get_id e), (get_ele e)) ((get_id e1), (get_ele e1)) (tolist s0)
-//   //                            ))));
-//   admit(); ()
+  assert(forall e e1. mem e (tolist s0) /\ (mem e1 (filter_s (fun e1 -> memq e s0 && memq e1 s0 && fst e <> fst e1) (tolist s0))) ==>
+                    (mem (fst e, Enqueue (snd e)) (enq_list) && mem (fst e1, Enqueue (snd e1)) (enq_list) && fst e <> fst e1 // &&
+                   //     ((tr.vis (fst e, Enqueue (snd e)) (fst e1, Enqueue (snd e1))) ||
+                   //       (not (tr.vis (fst e, Enqueue (snd e)) (fst e1, Enqueue (snd e1)) ||
+                   //              tr.vis (fst e1, Enqueue (snd e1)) (fst e, Enqueue (snd e))) &&
+                   // (fst e < fst e1)))
+  ));
+  admit(); ()
 
 // #set-options "--initial_fuel 10 --ifuel 10 --initial_ifuel 10 --fuel 10 --z3rlimit 1000000"
 
-// val prop_merge2 : ltr: ae
-//                 -> l:s
-//                 -> atr:ae
-//                 -> a:s
-//                 -> btr:ae
-//                 -> b:s
-//                 -> Lemma (requires ((forall e. mem e ltr.l ==> not (member (get_id e) atr.l)) /\
-//                                    (forall e. mem e ltr.l ==> not (member (get_id e) btr.l)) /\
-//                                    (forall e. mem e atr.l ==> not (member (get_id e) btr.l)) /\
-//                                    (forall e e1. (memq e a /\ memq e1 l /\ (fst e = fst e1)) ==> (snd e = snd e1)) /\
-//                                    (forall e e1. (memq e b /\ memq e1 l /\ (fst e = fst e1)) ==> (snd e = snd e1)) /\
-//                                    (forall e e1. (mem e ltr.l /\ mem e1 atr.l ==> get_id e < get_id e1)) /\
-//                                    (forall e e1. (mem e ltr.l /\ mem e1 btr.l ==> get_id e < get_id e1)) /\
-//                                    (sim ltr l /\ sim (union ltr atr) a /\ sim (union ltr btr) b) /\
-//                                    (forall e. mem_id e (diff_s (tolist a) (tolist l)) ==> not (mem_id e (diff_s (tolist b) (tolist l)))) /\
-//                                    (forall e. mem_id e (diff_s (tolist b) (tolist l)) ==> not (mem_id e (diff_s (tolist a) (tolist l))))))
-//                        (ensures (sim2 (absmerge ltr atr btr) (merge ltr l atr a btr b)))
+val prop_merge2 : ltr: ae
+                -> l:s
+                -> atr:ae
+                -> a:s
+                -> btr:ae
+                -> b:s
+                -> Lemma (requires ((forall e. mem e ltr.l ==> not (member (get_id e) atr.l)) /\
+                                   (forall e. mem e ltr.l ==> not (member (get_id e) btr.l)) /\
+                                   (forall e. mem e atr.l ==> not (member (get_id e) btr.l)) /\
+                                   (forall e e1. (memq e a /\ memq e1 l /\ (fst e = fst e1)) ==> (snd e = snd e1)) /\
+                                   (forall e e1. (memq e b /\ memq e1 l /\ (fst e = fst e1)) ==> (snd e = snd e1)) /\
+                                   (forall e e1. (mem e ltr.l /\ mem e1 atr.l ==> get_id e < get_id e1)) /\
+                                   (forall e e1. (mem e ltr.l /\ mem e1 btr.l ==> get_id e < get_id e1)) /\
+                                   (sim ltr l /\ sim (union ltr atr) a /\ sim (union ltr btr) b) /\
+                                   (forall e. mem_id e (diff_s (tolist a) (tolist l)) ==> not (mem_id e (diff_s (tolist b) (tolist l)))) /\
+                                   (forall e. mem_id e (diff_s (tolist b) (tolist l)) ==> not (mem_id e (diff_s (tolist a) (tolist l))))))
+                       (ensures (sim2 (absmerge ltr atr btr) (merge ltr l atr a btr b)))
 
-// let prop_merge2 ltr l atr a btr b =
-//   axiom_ae ltr; axiom_ae atr; axiom_ae btr; axiom_ae (union ltr atr); axiom_ae (union ltr btr);
-//   prop_merge01 ltr l atr a btr b; prop_merge0 ltr l atr a btr b; ()
+let prop_merge2 ltr l atr a btr b =
+  axiom_ae ltr; axiom_ae atr; axiom_ae btr; axiom_ae (union ltr atr); axiom_ae (union ltr btr);
+  prop_merge01 ltr l atr a btr b; prop_merge0 ltr l atr a btr b; ()
 
-// val prop_merge : ltr: ae
-//                 -> l:s
-//                 -> atr:ae
-//                 -> a:s
-//                 -> btr:ae
-//                 -> b:s
-//                 -> Lemma (requires ((forall e. mem e ltr.l ==> not (member (get_id e) atr.l)) /\
-//                                    (forall e. mem e ltr.l ==> not (member (get_id e) btr.l)) /\
-//                                    (forall e. mem e atr.l ==> not (member (get_id e) btr.l)) /\
-//                                    (forall e e1. (mem e ltr.l /\ mem e1 atr.l ==> get_id e < get_id e1)) /\
-//                                    (forall e e1. (mem e ltr.l /\ mem e1 btr.l ==> get_id e < get_id e1)) /\
-//                                    (sim ltr l /\ sim (union ltr atr) a /\ sim (union ltr btr) b) /\
-//                                    (forall e. mem_id e (diff_s (tolist a) (tolist l)) ==> not (mem_id e (diff_s (tolist b) (tolist l))))/\
-//                                    (forall e. mem_id e (diff_s (tolist b) (tolist l)) ==> not (mem_id e (diff_s (tolist a) (tolist l))))))
-//                        (ensures (sim (absmerge ltr atr btr) (merge ltr l atr a btr b)))
-// let prop_merge ltr l atr a btr b =
-//   prop_merge0 ltr l atr a btr b;
-//   prop_merge1 ltr l atr a btr b;
-//   prop_merge2 ltr l atr a btr b; ()
+val prop_merge : ltr: ae
+                -> l:s
+                -> atr:ae
+                -> a:s
+                -> btr:ae
+                -> b:s
+                -> Lemma (requires ((forall e. mem e ltr.l ==> not (member (get_id e) atr.l)) /\
+                                   (forall e. mem e ltr.l ==> not (member (get_id e) btr.l)) /\
+                                   (forall e. mem e atr.l ==> not (member (get_id e) btr.l)) /\
+                                   (forall e e1. (mem e ltr.l /\ mem e1 atr.l ==> get_id e < get_id e1)) /\
+                                   (forall e e1. (mem e ltr.l /\ mem e1 btr.l ==> get_id e < get_id e1)) /\
+                                   (sim ltr l /\ sim (union ltr atr) a /\ sim (union ltr btr) b) /\
+                                   (forall e. mem_id e (diff_s (tolist a) (tolist l)) ==> not (mem_id e (diff_s (tolist b) (tolist l))))/\
+                                   (forall e. mem_id e (diff_s (tolist b) (tolist l)) ==> not (mem_id e (diff_s (tolist a) (tolist l))))))
+                       (ensures (sim (absmerge ltr atr btr) (merge ltr l atr a btr b)))
+let prop_merge ltr l atr a btr b =
+  prop_merge0 ltr l atr a btr b;
+  prop_merge1 ltr l atr a btr b;
+  prop_merge2 ltr l atr a btr b; ()
 
 
 val convergence : tr:ae
